src/Computation/FixComp.v
@@ -2,204 +2,422 @@ Require Import
         Coq.Sets.Ensembles
         Coq.Classes.Morphisms
         Coq.Classes.SetoidTactics
-        Fiat.Computation.
+        Fiat.Computation
+        Fiat.Computation.SetoidMorphisms.
 
-Section FixComp.
+Record funSig :=
+  { funDom : list Type;
+    funCod : Type }.
 
-  Record funSig :=
-    { funDom : list Type;
-      funCod : Type }.
+Fixpoint funType
+         (fDom : list Type)
+         (fCod : Type)
+         {struct fDom}
+  : Type :=
+  match fDom with
+  | nil => Comp fCod
+  | cons T fDom' => T -> funType fDom' fCod
+  end.
 
-  Fixpoint funType
-           (fDom : list Type)
-           (fCod : Type)
-           {struct fDom}
-    : Type :=
-    match fDom with
-    | nil => Comp fCod
-    | cons T fDom' => T -> funType fDom' fCod
-    end.
+Fixpoint cfunType
+         (fDom : list Type)
+         (fCod : Type)
+         {struct fDom}
+  : Type :=
+  match fDom with
+  | nil => fCod
+  | cons T fDom' => T -> cfunType fDom' fCod
+  end.
 
-  Fixpoint cfunType
-           (fDom : list Type)
-           (fCod : Type)
-           {struct fDom}
-    : Type :=
-    match fDom with
-    | nil => fCod
-    | cons T fDom' => T -> cfunType fDom' fCod
-    end.
+Definition funDef (fSig : funSig) :=
+  funType (funDom fSig) (funCod fSig).
 
-  Definition funDef (fSig : funSig) :=
-    funType (funDom fSig) (funCod fSig).
+Fixpoint refineFun
+         {fDom : list Type}
+         {fCod : Type}
+         (fSet' fSet : funType fDom fCod)
+         {struct fDom} : Prop :=
+  match fDom as fDom' return
+        funType fDom' fCod
+        -> funType fDom' fCod
+        -> Prop
+  with
+  | nil =>
+    fun fSet' fSet => refine fSet' fSet
+  | cons T fDom' =>
+    fun fSet' fSet =>
+      forall (t : T), refineFun (fSet' t) (fSet t)
+  end fSet' fSet.
 
-  Fixpoint refineFun
+Lemma refineFun_refl
+      {fDom : list Type}
+      {fCod : Type}
+  : forall (fDef : funType fDom fCod),
+    refineFun fDef fDef.
+Proof.
+  induction fDom; simpl; intros.
+  - reflexivity.
+  - eauto.
+Qed.
+
+Lemma refineFun_trans
+      {fDom : list Type}
+      {fCod : Type}
+  : forall (fDef fDef' fDef'' : funType fDom fCod),
+    refineFun fDef fDef'
+    -> refineFun fDef' fDef''
+    -> refineFun fDef fDef''.
+Proof.
+  induction fDom; simpl; intros.
+  - rewrite H; eauto.
+  - eauto.
+Qed.
+
+Definition refineEquivFun
            {fDom : list Type}
            {fCod : Type}
            (fSet' fSet : funType fDom fCod)
-           {struct fDom} : Prop :=
-    match fDom as fDom' return
-          funType fDom' fCod
-          -> funType fDom' fCod
-          -> Prop
-    with
-    | nil =>
-      fun fSet' fSet => refine fSet' fSet
-    | cons T fDom' =>
-      fun fSet' fSet =>
-        forall (t : T), refineFun (fSet' t) (fSet t)
-    end fSet' fSet.
+  : Prop :=
+  refineFun fSet fSet' /\ refineFun fSet' fSet.
 
-  Definition FixedPointP
-             {fDom : list Type}
-             {fCod : Type}
-             (fDef : funType fDom fCod -> funType fDom fCod)
-             (fSet : funType fDom fCod)
-    : Prop :=
-    refineFun (fDef fSet) fSet /\ refineFun fSet (fDef fSet).
+Fixpoint FunMax
+         {fDom : list Type}
+         {fCod : Type}
+         (fSet' fSet : funType fDom fCod)
+         {struct fDom} : funType fDom fCod :=
+  match fDom as fDom' return
+        funType fDom' fCod
+        -> funType fDom' fCod
+        -> funType fDom' fCod
+  with
+  | nil =>
+    fun fSet' fSet => @Intersection _ fSet' fSet
+  | cons T fDom' =>
+    fun fSet' fSet =>
+      (fun (t : T) => FunMax (fSet' t) (fSet t))
+  end fSet' fSet.
 
-  Definition LeastFixedPointP
-             {fDom : list Type}
-             {fCod : Type}
-             (fDef : funType fDom fCod -> funType fDom fCod)
-             (fSet : funType fDom fCod)
-    : Prop :=
-    FixedPointP fDef fSet /\
-    forall fSet', FixedPointP fDef fSet'
-                  -> refineFun fSet' fSet.
+Fixpoint FunMin
+         {fDom : list Type}
+         {fCod : Type}
+         (fSet' fSet : funType fDom fCod)
+         {struct fDom} : funType fDom fCod :=
+  match fDom as fDom' return
+        funType fDom' fCod
+        -> funType fDom' fCod
+        -> funType fDom' fCod
+  with
+  | nil =>
+    fun fSet' fSet => @Union _ fSet' fSet
+  | cons T fDom' =>
+    fun fSet' fSet =>
+      (fun (t : T) => FunMin (fSet' t) (fSet t))
+  end fSet' fSet.
+
+Module LeastFixedPointFun.
+  Require Import Fiat.Common.Frame.
+
+  Instance funDefOps
+           {fDom : list Type}
+           {fCod : Type}
+    : Fiat.Common.Frame.Lattice.Ops (funType fDom fCod) :=
+    { le := refineFun;
+      eq := refineEquivFun;
+      max := FunMax;
+      min := FunMin
+    }.
+
+  Instance LatticeFun
+           {fDom : list Type}
+           {fCod : Type}
+    : Fiat.Common.Frame.Lattice.t (funType fDom fCod) funDefOps.
+
+  Instance PreO_refineFun
+           {fDom : list Type}
+           {fCod : Type}
+    : PreO.t (@refineFun fDom fCod) :=
+    { le_refl := refineFun_refl;
+      le_trans := refineFun_trans }.
+
+  Lemma refineFun_Proper
+        {fDom : list Type}
+        {fCod : Type}
+    : Proper (refineEquivFun ==> refineEquivFun ==> iff)
+             (@refineFun fDom fCod).
+  Proof.
+    unfold Proper, respectful; intros.
+    destruct H; destruct H0; intuition intros.
+    eapply refineFun_trans; eauto.
+    eapply refineFun_trans; eauto.
+    eapply refineFun_trans; eauto.
+    eapply refineFun_trans; eauto.
+  Qed.
+
+  Lemma refineFun_antisym
+        {fDom : list Type}
+        {fCod : Type}
+    : forall (x y : funType fDom fCod),
+      refineFun x y -> refineFun y x ->
+      refineEquivFun x y.
+  Proof.
+    unfold refineEquivFun; intuition.
+  Qed.
+
+  Instance PO_refineFun
+           {fDom : list Type}
+           {fCod : Type}
+    : PO.t (@refineFun fDom fCod) refineEquivFun :=
+    { PreO := PreO_refineFun;
+      le_proper := refineFun_Proper;
+      le_antisym := refineFun_antisym}.
 
   Local Transparent computes_to.
 
-  (*
-  Definition LeastFixedPoint {A}
-             (f : Comp A -> Comp A)
-    : Comp A :=
-    fun a =>
-      forall (ca : Comp A),
-        refine ca (f ca)
-        -> In _ ca a.
-
-  Lemma refine_LeastFixedPoint {A}
-    : forall (f : Comp A -> Comp A)
-             (f_monotone : forall rec rec',
-                 refine rec rec'
-                 -> refine (f rec) (f rec')),
-      refineEquiv (f (LeastFixedPoint f)) (LeastFixedPoint f).
-  Proof.
-    split; eauto.
-    unfold LeastFixedPoint, refine, computes_to in *; intros.
-    apply H0.
-    eapply f_monotone.
-    unfold computes_to.
-    apply f_monotone in H.
-
-    eapply f_monotone in H.
-
-    intros v' Comp_v'.
-    apply Comp_v'.
-    unfold computes_to in H.
-    apply H.
-    split; unfold refine; intros.
-
-
-
-
-  Defined.
-
-  Fixpoint LeastFixedPointFun'
-           (fDom : list Type)
-           {fCod : Type}
-           {struct fDom}
-    : (funType fDom fCod -> funType fDom fCod) -> funType fDom fCod.
-    refine match fDom return
-          (funType fDom fCod -> funType fDom fCod)
-          -> funType fDom fCod with
-    | nil => fun fDef => LeastFixedPoint fDef
-    | cons T fDom' =>
-      fun fDef (t : T) => LeastFixedPointFun' fDom' fCod _
-           end.
-    simpl in *.
-    intros.
-    apply LeastFixedPointFun'.
-    intro.
-
-    apply fDef.
-    intros.
-    apply X.
-    apply t.
-  Defined.
-
-
-   Definition LeastFixedPointFun
-             {fDom : list Type}
-             {fCod : Type}
-             (fDef : funType fDom fCod -> funType fDom fCod)
-    : funType fDom fCod :=
-    LeastFixedPointFun' fDom fDef.
-
-  Lemma refine_LeastFixedPointFun
+  Lemma funMax_Proper
         {fDom : list Type}
         {fCod : Type}
-        (fDef fDef' : funType fDom fCod -> funType fDom fCod)
-      : respectful (@refineFun fDom fCod)
-                   (@refineFun fDom fCod)
-                   fDef fDef'
-        -> refineFun (LeastFixedPointFun fDef)
-                     (LeastFixedPointFun fDef').
+    : Proper (@refineEquivFun
+                fDom fCod
+                ==> @refineEquivFun fDom fCod
+                ==> @refineEquivFun fDom fCod)
+             FunMax.
   Proof.
-    induction fDom; simpl; intros.
-    - unfold LeastFixedPointFun; simpl in *.
-      unfold refine; intros v Comp_v; intuition.
-      unfold computes_to, LeastFixedPoint,
-      FixedPointP, respectful in *; simpl in *.
-      intros.
-      eapply H; eauto.
-      2: eapply (Comp_v ca).
-      reflexivity.
-    - simpl in *.
-      eapply IHfDom; eauto.
-      unfold respectful in *; intros.
-      eapply H.
-      intro.
-      apply H0.
+    unfold refineEquivFun, Proper, respectful; intuition.
+    - induction fDom; simpl in *.
+      + intros c Comp_v; destruct Comp_v.
+        apply H0 in H; apply H2 in H4;
+        constructor; eauto.
+      + intros. eapply IHfDom; eauto.
+    - induction fDom; simpl in *.
+      + intros c Comp_v; destruct Comp_v.
+        apply H1 in H; apply H3 in H4;
+        constructor; eauto.
+      + intros. eapply IHfDom; eauto.
   Qed.
 
+  Lemma funMin_Proper
+        {fDom : list Type}
+        {fCod : Type}
+    : Proper (@refineEquivFun
+                fDom fCod
+                ==> @refineEquivFun fDom fCod
+                ==> @refineEquivFun fDom fCod)
+             FunMin.
+  Proof.
+    unfold refineEquivFun, Proper, respectful; intuition.
+    - induction fDom; simpl in *.
+      + intros c Comp_v; destruct Comp_v.
+        * constructor; apply H0; auto.
+        * constructor 2; apply H2; auto.
+      + intros; eapply IHfDom; eauto.
+    - induction fDom; simpl in *.
+      + intros c Comp_v; destruct Comp_v.
+        * constructor; apply H1; auto.
+        * constructor 2; apply H3; auto.
+      + intros; eapply IHfDom; eauto.
+  Qed.
 
-*)
+  Lemma FunMax_ok
+        {fDom : list Type}
+        {fCod : Type}
+    : forall l r : funType fDom fCod,
+      PreO.max (le := refineFun) l r (FunMax l r).
+  Proof.
+    constructor.
+    - induction fDom; simpl in *.
+      + intros v Comp_v; destruct Comp_v; eauto.
+      + eauto.
+    - induction fDom; simpl in *.
+      + intros v Comp_v; destruct Comp_v; eauto.
+      + eauto.
+    - induction fDom; simpl in *.
+      + intros.
+        intros v Comp_v; econstructor.
+        * apply H; eauto.
+        * apply H0; eauto.
+      + intros; eapply IHfDom; eauto.
+  Qed.
 
-  Fixpoint LeastFixedPoint'
+  Lemma FunMin_ok
+        {fDom : list Type}
+        {fCod : Type}
+    : forall l r : funType fDom fCod,
+      PreO.min (le := refineFun) l r (FunMin l r).
+  Proof.
+    constructor.
+    - induction fDom; simpl in *.
+      + intros v Comp_v; econstructor; eauto.
+      + eauto.
+    - induction fDom; simpl in *.
+      + intros v Comp_v; econstructor 2; eauto.
+      + eauto.
+    - induction fDom; simpl in *.
+      + intros.
+        intros v Comp_v; destruct Comp_v.
+        * apply H; eauto.
+        * apply H0; eauto.
+      + intros; eapply IHfDom; eauto.
+  Qed.
+
+  Instance Lattice_funDef
+           {fDom : list Type}
+           {fCod : Type}
+    : Lattice.t _ (@funDefOps fDom fCod) :=
+    { PO := PO_refineFun;
+      max_proper := funMax_Proper;
+      max_ok := FunMax_ok;
+      min_proper := funMin_Proper;
+      min_ok := FunMin_ok
+    }.
+
+  Fixpoint refineFun_inf'
            (fDom : list Type)
            {fCod : Type}
            {struct fDom}
-    : ((funType fDom fCod -> Prop) -> Prop) ->  funType fDom fCod :=
+    : ((funType fDom fCod -> Prop) -> Prop) -> funType fDom fCod :=
     match fDom return
           ((funType fDom fCod -> Prop) -> Prop)
           -> funType fDom fCod with
     | nil => fun LFP_P v => (LFP_P (fun cv => computes_to cv v))
     | cons T fDom' =>
       fun LFP_P =>
-        fun (t : T) => LeastFixedPoint' fDom' (fun cv => LFP_P (fun cv' => cv (cv' t)))
+        fun (t : T) => refineFun_inf' fDom' (fun cv => LFP_P (fun cv' => cv (cv' t)))
     end.
 
-  Definition LeastFixedPoint''
+  Definition refineFun_inf
+             {fDom : list Type}
+             {fCod : Type}
+             (f : funType fDom fCod -> Prop)
+    : funType fDom fCod :=
+    refineFun_inf' fDom (fun z => (forall s, f s -> z s)).
+
+  Lemma lub_refineFun_inf
+             (fDom : list Type)
+             {fCod : Type}
+             (f : funType fDom fCod -> Prop)
+    : lub f (refineFun_inf f).
+  Proof.
+    unfold lub, refineFun_inf; simpl.
+    induction fDom.
+    - unfold lub; simpl in *.
+      unfold refineFun_inf; simpl.
+      intuition.
+      intros v Comp_v.
+      unfold computes_to in *.
+      eapply (Comp_v a'); eauto.
+      intros v Comp_v.
+      unfold computes_to in *.
+      intros; apply H; eauto.
+    - simpl in *.
+      unfold lub in *; simpl in *; intuition.
+      unfold refineFun_inf.
+  Admitted.
+
+  Definition refineFun_sup
+           {fDom : list Type}
+           {fCod : Type}
+           (f : funType fDom fCod -> Prop)
+    : funType fDom fCod :=
+    refineFun_inf' fDom (fun z => exists s, f s /\ z s).
+
+  Definition glb_refineFun_sup
+             (fDom : list Type)
+             {fCod : Type}
+             (f : funType fDom fCod -> Prop)
+    : glb f (refineFun_sup f).
+  Proof.
+    induction fDom.
+    - unfold glb; simpl in *.
+      unfold refineFun_sup; simpl.
+      intuition.
+      + intros v Comp_v.
+        unfold computes_to in *.
+        eexists a'; intuition.
+      + intros v Comp_v.
+        unfold computes_to in *.
+        destruct Comp_v as [? [? ? ] ].
+        eapply H in H0.
+        apply H0 in H1; eauto.
+    - simpl in *.
+
+      unfold glb in *; simpl in *; intuition.
+  Admitted.
+
+  Instance CompleteLattice_funDef
+           {fDom : list Type}
+           {fCod : Type}
+    :  CompleteLattice (O := @funDefOps fDom fCod) :=
+    { cl_sup := refineFun_sup;
+      cl_inf := refineFun_inf
+    }.
+  Proof.
+    eapply glb_refineFun_sup.
+    eapply lub_refineFun_inf.
+  Defined.
+
+  Definition LeastFixedPoint
              {fDom : list Type}
              {fCod : Type}
              (fDef : funType fDom fCod -> funType fDom fCod)
     : funType fDom fCod :=
-    LeastFixedPoint' fDom (fun z => exists s, LeastFixedPointP fDef s /\ z s).
+    (cl_sup (prefixed_point fDef)).
+
+  Instance PreOrder_refineFun
+           {fDom : list Type}
+           {fCod : Type}
+    : PreOrder (@refineFun fDom fCod).
+  Proof.
+    constructor.
+    unfold Reflexive; apply refineFun_refl.
+    unfold Transitive; apply refineFun_trans.
+  Qed.
+
+  Lemma refine_LeastFixedPoint
+        {fDom : list Type}
+        {fCod : Type}
+        (fDef fDef' : funType fDom fCod -> funType fDom fCod)
+      : respectful (@refineFun fDom fCod)
+                   (@refineFun fDom fCod)
+                   fDef fDef'
+        ->
+        forall (fDef_monotone : forall rec rec',
+                   refineFun rec rec'
+                   -> refineFun (fDef rec) (fDef rec'))
+               (fDef'_monotone : forall rec rec',
+                   refineFun rec rec'
+                   -> refineFun (fDef' rec) (fDef' rec')),
+        refineFun (LeastFixedPoint fDef)
+                     (LeastFixedPoint fDef').
+  Proof.
+    unfold LeastFixedPoint, respectful; intros.
+    destruct (sup_glb (prefixed_point fDef)) as [? ?];
+      destruct (sup_glb (prefixed_point fDef')) as [? ?];
+      simpl in *.
+    eapply refineFun_trans.
+    eapply (H0 (fDef (refineFun_sup (prefixed_point fDef')))).
+    eapply fDef_monotone.
+    eapply refineFun_trans.
+    eapply H.
+    eapply refineFun_refl.
+    pose proof (proj2 (Is_LeastFixedPoint (O := @funDefOps fDom fCod) _ (fDef'_monotone))); eapply H4.
+    eapply refineFun_trans.
+    eapply H.
+    eapply refineFun_refl.
+    pose proof (proj2 (Is_LeastFixedPoint (O := @funDefOps fDom fCod) _ (fDef'_monotone))); eapply H4.
+  Qed.
 
   Definition FibonacciSpec
     : funType ((nat : Type) :: @nil Type)%list nat :=
-    LeastFixedPoint'' (fDom := (nat : Type) :: @nil Type)%list
-      (fun rec (n : nat) =>
-         match n with
-         | 0 => ret 0
-         | 1 => ret 1
-         | S (S n') =>
-           n1 <- rec n';
-           n2 <- rec (S n');
-           ret (n1 + n2)
-         end).
+    LeastFixedPoint (fDom := (nat : Type) :: @nil Type)%list
+                      (fun rec (n : nat) =>
+                         match n with
+                         | 0 => ret 0
+                         | 1 => ret 1
+                         | S (S n') =>
+                           n1 <- rec n';
+                             n2 <- rec (S n');
+                             ret (n1 + n2)
+                         end).
 
   Fixpoint FibonacciImpl
            (n : nat)
@@ -210,14 +428,19 @@ Section FixComp.
       match p with
       | 0 => ret 1
       | (S m) => n1 <- FibonacciImpl p;
-                 n2 <- FibonacciImpl m;
-                 ret (n1 + n2)
+                   n2 <- FibonacciImpl m;
+                   ret (n1 + n2)
       end
     end.
 
   Lemma foo
     : refineFun FibonacciSpec FibonacciImpl.
   Proof.
+    eapply refineFun_trans.
+    eapply refine_LeastFixedPoint; intros.
+    unfold respectful; simpl; intros.
+    Focus 3.
+
     unfold refineFun; unfold refine; intros.
     unfold FibonacciSpec, LeastFixedPoint''; simpl.
     unfold LeastFixedPointP, FixedPointP, computes_to; simpl.
@@ -228,7 +451,7 @@ Section FixComp.
     admit.
     admit.
   Admitted.
-  (*rewrite H1.
+(*rewrite H1.
     induction t0.
     - reflexivity.
     - simpl.
@@ -423,5 +646,5 @@ Section FixComp.
       intro.
       apply H0.
   Qed.
-   *)
+ *)
 End FixComp.
